Admit lemmas, ensure new fields for case studies/examples are added everywhere.

case_study/MinimalCaps/Machine.v
@@ -180,6 +180,8 @@ Section FunDeclKit.
 
   #[export] Instance 𝑭_eq_dec : EqDec (sigT (fun Γ => sigT (𝑭 Γ))) :=
     sigma_eqdec _ (fun Γ => sigma_eqdec _ (fun τ => _)).
+
+  Definition inline_fuel : nat := 10.
 End FunDeclKit.
 
 Include FunDeclMixin MinCapsBase.
@@ -923,166 +925,176 @@ End ForeignKit.
 Include ProgramMixin MinCapsBase.
 
 Section WellFoundedKit.
+
+  Lemma 𝑭_bind_free : ∀ {Δ τ} (f : 𝑭 Δ τ), BindFree inline_fuel (FunDef f).
+  Proof.
+    intros Δ τ f.
+    apply BindFreeBool_eq.
+    destruct f; auto.
+  Admitted.
+
   (* TODO: look more at other works, that might've run into something similar *)
-  Lemma 𝑭_well_founded : ∃ fuel, well_founded (InvokedByFunPackage fuel).
+  Lemma 𝑭_well_founded : well_founded (InvokedByFunPackage inline_fuel).
   Proof.
     (* TODO: need proof by reflection. Define a decidable impl of InvokedBy, so we can compute that well_founded holds. *)
-    exists 3.
     intros [Δ1 [τ1 f1]]. constructor. intros [Δ2 [τ2 f2]] Hinvok.
-    assert (InvokedByFunPackageBool 3 (existT _ (existT _ f2)) (existT _ (existT _ f1)) = true) as H.
-    { destruct (InvokedByFunPackage_spec 3 (existT _ (existT _ f2)) (existT _ (existT _ f1))); auto. }
+    assert (InvokedByFunPackageBool inline_fuel (existT _ (existT _ f2)) (existT _ (existT _ f1)) = true) as H.
+    {
+      destruct (InvokedByFunPackage_spec inline_fuel (existT _ (existT _ f2)) (existT _ (existT _ f1))); auto.
+      unfold BindFreeFunPackage, BindFreeFun. apply 𝑭_bind_free.
+    }
     unfold InvokedByFunPackageBool in H.
     unfold InvokedByFunBool in H.
     rewrite InvokedByStmWithFuelInListBool_eq in H.
-    assert (InvokedByStmWithFuelInList 3 f2 (FunDef f1)) as H'.
-    { destruct (InvokedByStmWithFuelInList_spec 3 f2 (FunDef f1)); auto.
+    assert (InvokedByStmWithFuelInList inline_fuel f2 (FunDef f1)) as H'.
+    { destruct (InvokedByStmWithFuelInList_spec inline_fuel f2 (FunDef f1)); auto.
       discriminate. }
     unfold InvokedByStmWithFuelInListBool in H.
     Time destruct f1, f2; cbv in H.
     all: try discriminate.
 
-    (* TODO: handle existsb better? *)
-    destruct f1;
-    match goal with
-    | H: context[InvokedByStmWithFuelList ?fuel ?f] |- _ =>
-        let l := (eval cbv in (InvokedByStmWithFuelList fuel f)) in
-        change (InvokedByStmWithFuelList fuel f) with l in H
-    end.
-    - admit.
-    - admit.
-    - admit.
-    - admit.
-    - admit.
-    - admit.
-    - admit.
-    - admit.
-    - admit.
-    - admit.
-    - admit.
-    - admit.
-    - admit.
-    - admit.
-    - admit.
-    - admit.
-    - admit.
-    - admit.
-    - admit.
-    - admit.
-    - admit.
-    - admit.
-    - admit.
-    - admit.
-    - admit.
-    - admit.
-    - admit.
-    - admit.
-    - admit.
-    - admit.
-    - admit.
-    - admit.
-    - admit.
-    - admit.
-    - admit.
-    - admit.
-    - admit.
-    - admit.
-    - admit.
-    - admit.
-    - admit.
-    - admit.
-    - admit.
-    - admit.
-    - admit.
-    - admit.
-    - admit.
-    - admit.
-    - admit.
-    - admit.
-    - destruct f2; cbv in H; try discriminate.
+  (*   (* TODO: handle existsb better? *) *)
+  (*   destruct f1; *)
+  (*   match goal with *)
+  (*   | H: context[InvokedByStmWithFuelList ?fuel ?f] |- _ => *)
+  (*       let l := (eval cbv in (InvokedByStmWithFuelList fuel f)) in *)
+  (*       change (InvokedByStmWithFuelList fuel f) with l in H *)
+  (*   end. *)
+  (*   - admit. *)
+  (*   - admit. *)
+  (*   - admit. *)
+  (*   - admit. *)
+  (*   - admit. *)
+  (*   - admit. *)
+  (*   - admit. *)
+  (*   - admit. *)
+  (*   - admit. *)
+  (*   - admit. *)
+  (*   - admit. *)
+  (*   - admit. *)
+  (*   - admit. *)
+  (*   - admit. *)
+  (*   - admit. *)
+  (*   - admit. *)
+  (*   - admit. *)
+  (*   - admit. *)
+  (*   - admit. *)
+  (*   - admit. *)
+  (*   - admit. *)
+  (*   - admit. *)
+  (*   - admit. *)
+  (*   - admit. *)
+  (*   - admit. *)
+  (*   - admit. *)
+  (*   - admit. *)
+  (*   - admit. *)
+  (*   - admit. *)
+  (*   - admit. *)
+  (*   - admit. *)
+  (*   - admit. *)
+  (*   - admit. *)
+  (*   - admit. *)
+  (*   - admit. *)
+  (*   - admit. *)
+  (*   - admit. *)
+  (*   - admit. *)
+  (*   - admit. *)
+  (*   - admit. *)
+  (*   - admit. *)
+  (*   - admit. *)
+  (*   - admit. *)
+  (*   - admit. *)
+  (*   - admit. *)
+  (*   - admit. *)
+  (*   - admit. *)
+  (*   - admit. *)
+  (*   - admit. *)
+  (*   - admit. *)
+  (*   - destruct f2; cbv in H; try discriminate. *)
 
       
-    Time destruct f1; cbv in H. (* ~250s *)
-    Time destruct f1; cbn in H. (* ~250s *)
-    all: try discriminate.
-    - destruct f2; try discriminate.
-      constructor. intros f1 H''.
-      assert (InvokedByFunPackageBool 3 f1 (existT _ (existT _ read_reg)) = true) as H'''.
-      { destruct (InvokedByFunPackage_spec 3 f1 (existT _ (existT _ read_reg))); auto. }
-      unfold InvokedByFunPackageBool in H'''.
-      unfold InvokedByFunBool in H'''.
-      destruct f1 as [Δ [τ f1]].
-      rewrite InvokedByStmWithFuelInListBool_eq in H'''.
-      assert (InvokedByStmWithFuelInList 3 f1 (FunDef read_reg)) as H''''.
-      { destruct (InvokedByStmWithFuelInList_spec 3 f1 (FunDef read_reg)); auto.
-        discriminate. }
-      destruct f1; cbn in H''''; try discriminate.
-    - admit.
-    - admit.
-    - admit.
-    - admit.
-    - admit.
-    - admit.
-    - admit.
-    - admit.
-    - admit.
-    - admit.
-    - admit.
-    - admit.
-    - admit.
-    - admit.
-    - admit.
-    - admit.
-    - admit.
-    - admit.
-    - admit.
-    - admit.
-    - admit.
-    - admit.
-    - admit.
-    - admit.
-    - admit.
-    - admit.
-    - admit.
-    - admit.
-    - admit.
-    - admit.
-    - admit.
-    - admit.
-    - admit.
-    - admit.
-    - destruct f2; cbn in H; try discriminate.
-      admit.
-      admit.
-      admit.
-      admit.
-      admit.
-      admit.
-      admit.
-      admit.
-      admit.
-      admit.
-      admit.
-      admit.
-      admit.
-      admit.
-      admit.
-      admit.
-      admit.
-      admit.
-      admit.
-      admit.
-      admit.
-      admit.
-      admit.
-      admit.
-      admit.
-      admit.
-      admit.
-      admit.
-      admit.
-      admit.
-      admit.
-      admit.
+  (*   Time destruct f1; cbv in H. (* ~250s *) *)
+  (*   Time destruct f1; cbn in H. (* ~250s *) *)
+  (*   all: try discriminate. *)
+  (*   - destruct f2; try discriminate. *)
+  (*     constructor. intros f1 H''. *)
+  (*     assert (InvokedByFunPackageBool 3 f1 (existT _ (existT _ read_reg)) = true) as H'''. *)
+  (*     { destruct (InvokedByFunPackage_spec 3 f1 (existT _ (existT _ read_reg))); auto. } *)
+  (*     unfold InvokedByFunPackageBool in H'''. *)
+  (*     unfold InvokedByFunBool in H'''. *)
+  (*     destruct f1 as [Δ [τ f1]]. *)
+  (*     rewrite InvokedByStmWithFuelInListBool_eq in H'''. *)
+  (*     assert (InvokedByStmWithFuelInList 3 f1 (FunDef read_reg)) as H''''. *)
+  (*     { destruct (InvokedByStmWithFuelInList_spec 3 f1 (FunDef read_reg)); auto. *)
+  (*       discriminate. } *)
+  (*     destruct f1; cbn in H''''; try discriminate. *)
+  (*   - admit. *)
+  (*   - admit. *)
+  (*   - admit. *)
+  (*   - admit. *)
+  (*   - admit. *)
+  (*   - admit. *)
+  (*   - admit. *)
+  (*   - admit. *)
+  (*   - admit. *)
+  (*   - admit. *)
+  (*   - admit. *)
+  (*   - admit. *)
+  (*   - admit. *)
+  (*   - admit. *)
+  (*   - admit. *)
+  (*   - admit. *)
+  (*   - admit. *)
+  (*   - admit. *)
+  (*   - admit. *)
+  (*   - admit. *)
+  (*   - admit. *)
+  (*   - admit. *)
+  (*   - admit. *)
+  (*   - admit. *)
+  (*   - admit. *)
+  (*   - admit. *)
+  (*   - admit. *)
+  (*   - admit. *)
+  (*   - admit. *)
+  (*   - admit. *)
+  (*   - admit. *)
+  (*   - admit. *)
+  (*   - admit. *)
+  (*   - admit. *)
+  (*   - destruct f2; cbn in H; try discriminate. *)
+  (*     admit. *)
+  (*     admit. *)
+  (*     admit. *)
+  (*     admit. *)
+  (*     admit. *)
+  (*     admit. *)
+  (*     admit. *)
+  (*     admit. *)
+  (*     admit. *)
+  (*     admit. *)
+  (*     admit. *)
+  (*     admit. *)
+  (*     admit. *)
+  (*     admit. *)
+  (*     admit. *)
+  (*     admit. *)
+  (*     admit. *)
+  (*     admit. *)
+  (*     admit. *)
+  (*     admit. *)
+  (*     admit. *)
+  (*     admit. *)
+  (*     admit. *)
+  (*     admit. *)
+  (*     admit. *)
+  (*     admit. *)
+  (*     admit. *)
+  (*     admit. *)
+  (*     admit. *)
+  (*     admit. *)
+  (*     admit. *)
+  (*     admit. *)
   Admitted.
 
 End WellFoundedKit.
