test/LinkedList.v
@@ -142,9 +142,10 @@ Module Import ExampleProgram <: Program ExampleBase.
 
     Definition 𝑳 : PCtx -> Set := Lem.
 
-
     #[export] Instance 𝑭_eq_dec : EqDec (sigT (fun Γ => sigT (𝑭 Γ))).
     Admitted. (* TODO: solve *)
+
+    Definition inline_fuel : nat := 10.
   End FunDeclKit.
 
   (* A mixin provided by the library pulling in definitions of statements etc.
@@ -336,7 +337,7 @@ Module Import ExampleProgram <: Program ExampleBase.
 
   Section WellFoundedKit.
     (* TODO: solve *)
-    Lemma 𝑭_well_founded : exists fuel, well_founded (InvokedByFunPackage fuel).
+    Lemma 𝑭_well_founded : well_founded (InvokedByFunPackage inline_fuel).
     Admitted.
   End WellFoundedKit.
 End ExampleProgram.
