case_study/RiscvPmp/BinaryBlockVer/Verifier.v
@@ -1,0 +1,787 @@
+(******************************************************************************)
+(* Copyright (c) 2020 Steven Keuchel, Dominique Devriese, Sander Huyghebaert  *)
+(* All rights reserved.                                                       *)
+(*                                                                            *)
+(* Redistribution and use in source and binary forms, with or without         *)
+(* modification, are permitted provided that the following conditions are     *)
+(* met:                                                                       *)
+(*                                                                            *)
+(* 1. Redistributions of source code must retain the above copyright notice,  *)
+(*    this list of conditions and the following disclaimer.                   *)
+(*                                                                            *)
+(* 2. Redistributions in binary form must reproduce the above copyright       *)
+(*    notice, this list of conditions and the following disclaimer in the     *)
+(*    documentation and/or other materials provided with the distribution.    *)
+(*                                                                            *)
+(* THIS SOFTWARE IS PROVIDED BY THE COPYRIGHT HOLDERS AND CONTRIBUTORS        *)
+(* "AS IS" AND ANY EXPRESS OR IMPLIED WARRANTIES, INCLUDING, BUT NOT LIMITED  *)
+(* TO, THE IMPLIED WARRANTIES OF MERCHANTABILITY AND FITNESS FOR A PARTICULAR *)
+(* PURPOSE ARE DISCLAIMED. IN NO EVENT SHALL THE COPYRIGHT HOLDER OR          *)
+(* CONTRIBUTORS BE LIABLE FOR ANY DIRECT, INDIRECT, INCIDENTAL, SPECIAL,      *)
+(* EXEMPLARY, OR CONSEQUENTIAL DAMAGES (INCLUDING, BUT NOT LIMITED TO,        *)
+(* PROCUREMENT OF SUBSTITUTE GOODS OR SERVICES; LOSS OF USE, DATA, OR         *)
+(* PROFITS; OR BUSINESS INTERRUPTION) HOWEVER CAUSED AND ON ANY THEORY OF     *)
+(* LIABILITY, WHETHER IN CONTRACT, STRICT LIABILITY, OR TORT (INCLUDING       *)
+(* NEGLIGENCE OR OTHERWISE) ARISING IN ANY WAY OUT OF THE USE OF THIS         *)
+(* SOFTWARE, EVEN IF ADVISED OF THE POSSIBILITY OF SUCH DAMAGE.               *)
+(******************************************************************************)
+
+From Coq Require Import
+     Classes.Morphisms_Prop
+     ZArith.ZArith
+     Lists.List
+     micromega.Lia
+     Strings.String.
+From Equations Require Import
+     Equations.
+From Katamaran Require Import
+     Iris.Instance
+     Iris.Base
+     Notations
+     Semantics
+     Bitvector
+     Refinement.Monads
+     Sep.Hoare
+     Specification
+     Symbolic.Propositions
+     Symbolic.Solver
+     Symbolic.Worlds
+     MicroSail.ShallowExecutor
+     MicroSail.ShallowSoundness
+     MicroSail.SymbolicExecutor
+     MicroSail.RefineExecutor
+     MicroSail.Soundness
+     RiscvPmp.BlockVer.Spec
+     RiscvPmp.IrisModel
+     RiscvPmp.IrisInstance
+     RiscvPmp.Machine
+     RiscvPmp.Sig.
+From iris.base_logic Require lib.gen_heap lib.iprop invariants.
+From iris.bi Require interface big_op.
+From iris.algebra Require dfrac.
+From iris.program_logic Require total_weakestpre adequacy.
+From iris.proofmode Require string_ident tactics.
+From stdpp Require namespaces.
+
+Import RiscvPmpProgram.
+
+Set Implicit Arguments.
+Import ctx.resolution.
+Import ctx.notations.
+Import env.notations.
+Import ListNotations.
+Open Scope string_scope.
+Open Scope ctx_scope.
+Open Scope Z_scope.
+
+Import RiscvPmpIrisBase RiscvPmpIrisInstance.
+#[local] Notation "a '↦' t" := (reg_pointsTo a t) (at level 70).
+#[local] Notation "a '↦ₘ' t" := (interp_ptsto a t) (at level 70).
+
+Module ns := stdpp.namespaces.
+
+(*   Definition pmp_entry_cfg := ty_prod ty_pmpcfg_ent ty_xlenbits. *)
+
+Section BlockVerificationDerived.
+
+  Import RiscvPmpBlockVerifExecutor.
+  Import RiscvPmpBlockVerifShalExecutor.
+
+  Definition safeE {Σ} : 𝕊 Σ -> Prop :=
+    fun P => VerificationConditionWithErasure (Erasure.erase_symprop P).
+
+  Definition safeE_safe (p : 𝕊 wnil) (ι : Valuation wnil) : safeE p -> SymProp.safe p [].
+  Proof.
+    unfold safeE.
+    destruct 1 as [H].
+    now apply Erasure.erase_safe'.
+  Qed.
+
+  Section Symbolic.
+
+    Import ModalNotations.
+    Import SStoreSpec (evalStoreSpec).
+    Import SHeapSpec SHeapSpec.notations.
+    Import asn.notations.
+
+    Definition exec_instruction_prologue (i : AST) :
+      Assertion ([ctx] ▻ ("a":: ty_xlenbits)) :=
+      pc     ↦ term_var "a" ∗
+      asn.chunk (chunk_user ptstoinstr [term_var "a"; term_val ty_ast i]) ∗
+      asn.exist "an" ty_xlenbits (nextpc ↦ term_var "an").
+
+    Definition exec_instruction_epilogue (i : AST) :
+      Assertion ([ctx] ▻ ("a":: ty_xlenbits) ▻ ("an":: ty_xlenbits)) :=
+      pc     ↦ term_var "an" ∗
+      asn.chunk (chunk_user ptstoinstr [term_var "a"; term_val ty_ast i]) ∗
+      nextpc ↦ term_var "an".
+
+    Definition sexec_instruction (i : AST) :
+      ⊢ STerm ty_xlenbits -> SHeapSpec (STerm ty_xlenbits) :=
+      let inline_fuel := 10%nat in
+      fun _ a =>
+        ⟨ θ1 ⟩ _  <- produce
+                       (exec_instruction_prologue i)
+                       [env].["a"∷_ ↦ a] ;;
+        ⟨ θ2 ⟩ _  <- evalStoreSpec (sexec default_config inline_fuel (FunDef step) _) [env] ;;
+        ⟨ θ3 ⟩ na <- angelic None _ ;;
+        let a3 := persist__term a (θ1 ∘ θ2 ∘ θ3) in
+        ⟨ θ4 ⟩ _  <- consume
+                       (exec_instruction_epilogue i)
+                       [env].["a"∷_ ↦ a3].["an"∷_ ↦ na] ;;
+        pure (persist__term na θ4).
+
+    Fixpoint sexec_block_addr (b : list AST) :
+      ⊢ STerm ty_xlenbits -> STerm ty_xlenbits -> SHeapSpec (STerm ty_xlenbits) :=
+      fun _ ainstr apc =>
+        match b with
+        | nil       => pure apc
+        | cons i b' =>
+            ⟨ θ1 ⟩ _    <- assert_formula (fun _ => amsg.empty)
+                             (formula_relop bop.eq ainstr apc) ;;
+            ⟨ θ2 ⟩ apc' <- sexec_instruction i (persist__term apc θ1) ;;
+            sexec_block_addr b'
+              (term_binop bop.bvadd
+                 (persist__term ainstr (θ1 ∘ θ2))
+                 (term_val ty_word bv_instrsize))
+              apc'
+        end.
+
+    Definition sexec_double_addr {Σ : LCtx}
+      (req : Assertion (Σ ▻ ("a":: ty_xlenbits))) (b : list AST) :
+      ⊢ SHeapSpec (STerm ty_xlenbits) :=
+      fun _ =>
+        ⟨ θ1 ⟩ lenv1 <- demonic_ctx id Σ ;;
+        ⟨ θ2 ⟩ a2    <- demonic (Some "a") _ ;;
+        let lenv2 := env.snoc (persist (A := Sub Σ) lenv1 θ2) _ a2 in
+        ⟨ θ3 ⟩ _     <- produce req lenv2 ;;
+        let a3 := persist__term a2 θ3 in
+        sexec_block_addr b a3 a3.
+
+    Definition sexec_triple_addr {Σ : LCtx}
+      (req : Assertion (Σ ▻ ("a"::ty_xlenbits))) (b : list AST)
+      (ens : Assertion (Σ ▻ ("a"::ty_xlenbits) ▻ ("an"::ty_xlenbits))) :
+      ⊢ SHeapSpec Unit :=
+      fun w =>
+        ⟨ θ0 ⟩ δ <- demonic_ctx id Σ ;;
+        ⟨ θ1 ⟩ a <- demonic (Some "a") _ ;;
+        let δ1 := env.snoc (persist ( A:= Sub Σ) δ θ1) _ a in
+        ⟨ θ2 ⟩ _ <- produce req δ1 ;;
+        let a2 := persist__term a θ2 in
+        ⟨ θ3 ⟩ na <- sexec_block_addr b a2 a2 ;;
+        let δ3 := persist δ1 (θ2 ∘ θ3) in
+        consume ens δ3.["an"∷ty_xlenbits ↦ na].
+
+    (* This is a VC for triples, for doubles we probably need to talk
+       about the continuation of a block. *)
+    Definition sblock_verification_condition {Σ : LCtx}
+      (req : Assertion (Σ ▻ "a"∷ty_xlenbits)) (b : list AST)
+      (ens : Assertion (Σ ▻ "a"∷ty_xlenbits ▻ "an"∷ty_xlenbits)) : ⊢ 𝕊 :=
+      fun w =>
+        (* SHeapSpec does not perform a leakcheck. We could include one here. *)
+        SHeapSpec.run (sexec_triple_addr req b ens (w := w)).
+
+  End Symbolic.
+
+  Section Shallow.
+
+    Import CStoreSpec (evalStoreSpec).
+    Import CHeapSpec CHeapSpec.notations.
+
+    Definition cexec_instruction (i : AST) :
+      Val ty_xlenbits -> CHeapSpec (Val ty_xlenbits) :=
+      let inline_fuel := 10%nat in
+      fun a =>
+        _ <- produce
+               (exec_instruction_prologue i)
+               [env].["a"∷_ ↦ a] ;;
+        _ <- evalStoreSpec (cexec inline_fuel (FunDef step)) [env] ;;
+        na <- angelic _ ;;
+        _ <- consume
+               (exec_instruction_epilogue i)
+               [env].["a"∷ty_xlenbits ↦ a].["an"∷_ ↦ na] ;;
+        pure na.
+
+    Fixpoint cexec_block_addr (b : list AST) :
+      Val ty_xlenbits -> Val ty_xlenbits -> CHeapSpec (Val ty_xlenbits) :=
+      fun ainstr apc =>
+        match b with
+        | nil       => pure apc
+        | cons i b' =>
+            _ <- assert_formula (ainstr = apc) ;;
+            apc' <- cexec_instruction i apc ;;
+            cexec_block_addr b' (bv.add ainstr bv_instrsize) apc'
+        end.
+
+    Definition cexec_double_addr {Σ : LCtx}
+      (req : Assertion (Σ ▻ "a"∷ty_xlenbits)) (b : list AST) :
+      CHeapSpec (Val ty_xlenbits) :=
+      δ <- demonic_ctx Σ ;;
+      an <- demonic _ ;;
+      _ <- produce req δ.["a"∷ty_xlenbits ↦ an] ;;
+      cexec_block_addr b an an.
+
+    Definition cexec_triple_addr {Σ : LCtx}
+      (req : Assertion (Σ ▻ "a"∷ty_xlenbits)) (b : list AST)
+      (ens : Assertion (Σ ▻ "a"∷ty_xlenbits ▻ "an"∷ty_xlenbits)) :
+      CHeapSpec unit :=
+      lenv <- demonic_ctx Σ ;;
+      a    <- demonic _ ;;
+      _    <- produce req lenv.["a"∷ty_xlenbits ↦ a]  ;;
+      na   <- cexec_block_addr b a a ;;
+      consume ens lenv.["a"∷ty_xlenbits ↦ a].["an"∷ty_xlenbits ↦ na].
+
+    Definition cblock_verification_condition {Σ : LCtx}
+      (req : Assertion (Σ ▻ "a"∷ty_xlenbits)) (b : list AST)
+      (ens : Assertion (Σ ▻ "a"∷ty_xlenbits ▻ "an"∷ty_xlenbits)) : Prop :=
+      (* CHeapSpec.run does not perform a leakcheck. We could include one here. *)
+      CHeapSpec.run (cexec_triple_addr req b ens).
+
+    Import (hints) CStoreSpec.
+
+    #[export] Instance mono_cexec_instruction {i a} :
+      Monotonic (MHeapSpec eq) (cexec_instruction i a).
+    Proof. typeclasses eauto. Qed.
+
+    #[export] Instance mono_cexec_block_addr {instrs ainstr apc} :
+      Monotonic (MHeapSpec eq) (cexec_block_addr instrs ainstr apc).
+    Proof. revert ainstr apc. induction instrs; cbn; typeclasses eauto. Qed.
+
+  End Shallow.
+
+  Section Relational.
+
+    Import iris.proofmode.tactics logicalrelation logicalrelation.notations.
+    Import RiscvPmpIrisInstanceWithContracts.StoreSpec.
+    Import RiscvPmpIrisInstanceWithContracts.
+    Import RiscvPmpSignature.HeapSpec.
+    Import RSolve HeapSpec.
+
+    Lemma rexec_instruction (i : AST) {w} :
+      ⊢ ℛ⟦RVal ty_xlenbits -> RHeapSpec (RVal ty_xlenbits)⟧
+          (cexec_instruction i)
+          (sexec_instruction (w := w) i).
+    Proof.
+      unfold cexec_instruction, sexec_instruction. rsolve.
+    Qed.
+
+    #[export] Instance refine_compat_exec_instruction {i : AST} {w} :
+      RefineCompat (RVal ty_xlenbits -> RHeapSpec (RVal ty_xlenbits))
+        (cexec_instruction i) w (sexec_instruction (w := w) i) _ :=
+      MkRefineCompat (rexec_instruction i).
+
+    Lemma rexec_block_addr (b : list AST) {w} :
+      ⊢ ℛ⟦RVal ty_xlenbits -> RVal ty_xlenbits -> RHeapSpec (RVal ty_xlenbits)⟧
+          (cexec_block_addr b)
+          (sexec_block_addr b (w := w)).
+    Proof.
+      iAssert (ℛ⟦□ᵣ (RVal ty_xlenbits -> RVal ty_xlenbits -> RHeapSpec (RVal ty_xlenbits))⟧
+                 (cexec_block_addr b)
+                 (fun w' θ => sexec_block_addr b (w := w'))) as "H".
+      {
+        iInduction b as [|*] "IHb"; cbn; rsolve.
+        iApply ("IHb" with "[] [$]").
+        now rsolve.
+      }
+      iApply (unconditionally_T with "H").
+    Qed.
+
+    Lemma rexec_triple_addr {Σ : LCtx}
+      (req : Assertion (Σ ▻ "a"∷ty_xlenbits)) (b : list AST)
+      (ens : Assertion (Σ ▻ "a"∷ty_xlenbits ▻ "an"∷ty_xlenbits)) {w} :
+      ⊢ ℛ⟦RHeapSpec RUnit⟧
+          (cexec_triple_addr req b ens)
+          (sexec_triple_addr req b ens (w := w)).
+    Proof.
+      unfold cexec_triple_addr, sexec_triple_addr.
+      rsolve.
+      iApply rexec_block_addr; rsolve.
+      rewrite !forgetting_trans.
+      iModIntro.
+      iModIntro.
+      rsolve.
+    Qed.
+
+    Lemma rblock_verification_condition {Σ : LCtx}
+      (req : Assertion (Σ ▻ "a"∷ty_xlenbits)) (b : list AST)
+      (ens : Assertion (Σ ▻ "a"∷ty_xlenbits ▻ "an"∷ty_xlenbits)) {w} :
+      ⊢ RSat LogicalSoundness.RProp (w := w)
+          (cblock_verification_condition req b ens)
+          (sblock_verification_condition req b ens w).
+    Proof.
+      unfold cblock_verification_condition, sblock_verification_condition.
+      rsolve.
+      iApply refine_run.
+      iApply rexec_triple_addr.
+    Qed.
+
+  End Relational.
+
+  Section Soundness.
+
+    Import iris.base_logic.lib.iprop iris.proofmode.tactics.
+    Import RiscvPmpIrisInstanceWithContracts.
+    Import ProgramLogic.
+    Import CHeapSpec.
+
+    Context {Σ} {GS : sailGS Σ}.
+
+    Fixpoint ptsto_instrs (a : Val ty_word) (instrs : list AST) : iProp Σ :=
+      match instrs with
+      | cons inst insts => (interp_ptsto_instr a inst ∗ ptsto_instrs (bv.add a bv_instrsize) insts)%I
+      | nil => True%I
+      end.
+    (* Arguments ptsto_instrs {Σ H} a%_Z_scope instrs%_list_scope : simpl never. *)
+
+    Definition semTripleOneInstrStep (PRE : iProp Σ) (instr : AST) (POST : Val ty_word -> iProp Σ) (a : Val ty_word) : iProp Σ :=
+      semTTriple [env] (PRE ∗ (∃ v, lptsreg nextpc v) ∗ lptsreg pc a ∗ interp_ptsto_instr a instr)
+        (FunDef RiscvPmpProgram.step)
+        (fun ret _ => (∃ an, lptsreg nextpc an ∗ lptsreg pc an ∗ POST an) ∗ interp_ptsto_instr a instr)%I.
+
+    Definition semTripleBlock (PRE : Val ty_word -> iProp Σ) (instrs : list AST) (POST : Val ty_word -> Val ty_word -> iProp Σ) : iProp Σ :=
+      (∀ a,
+         (PRE a ∗ pc ↦ a ∗ (∃ v, nextpc ↦ v) ∗ ptsto_instrs a instrs) -∗
+         (∀ an, pc ↦ an ∗ (∃ v, nextpc ↦ v) ∗ ptsto_instrs a instrs ∗ POST a an -∗ WP_loop) -∗
+         WP_loop)%I.
+    #[global] Arguments semTripleBlock PRE%_I instrs POST%_I.
+
+    Lemma sound_stm_aux {τ} {PRE} {s : Stm [ctx] τ} {POST} :
+      # inline_fuel ⦃ PRE ⦄ s; [env] ⦃ POST ⦄ → ⊢ semTTriple [env] PRE s POST.
+    Proof.
+      iIntros (Htrip) "PRE".
+      iApply sound_tstm; eauto using TforeignSemBlockVerif, lemSemBlockVerif.
+      - intros Δ σ f H. apply 𝑭_well_founded.
+      - iIntros "!>" (σs σ f H).
+        iApply TcontractsSound.
+    Qed.
+
+    Lemma sound_exec_instruction {instr} a Φ (h : SCHeap) :
+      cexec_instruction instr a Φ h ->
+      ⊢ semTripleOneInstrStep (interpret_scheap h) instr
+          (fun an => ∃ h' : SCHeap, interpret_scheap h' ∧ ⌜Φ an h'⌝) a.
+    Proof.
+      cbv [cexec_instruction exec_instruction_prologue bind produce demonic
+             produce_chunk lift_purespec CPureSpec.produce_chunk CPureSpec.pure
+             CPureSpec.demonic CStoreSpec.evalStoreSpec].
+      cbn - [consume].
+      iIntros (Hverif) "(Hheap & [%npc Hnpc] & Hpc & Hinstrs)".
+      specialize (Hverif npc). apply sound_cexec in Hverif.
+      iApply (semTWP_mono with "[-]").
+    (*   iApply (sound_tstm TforeignSemBlockVerif lemSemBlockVerif (ex_intro _ _ Hverif) with "[] [$]"). *)
+    (*   iApply TcontractsSound. *)
+    (*   iIntros ([v|m] _); last done; iIntros "(%h1 & Hh1 & %Htrip)". clear Hverif. *)
+    (*   destruct Htrip as [an Htrip]. *)
+    (*   iPoseProof (consume_sound _ _ Htrip with "Hh1") *)
+    (*     as "[(Hpc & $ & Han) (%h2 & Hh2 & %HΦ)]". *)
+    (*   iExists an. cbn. by iFrame. *)
+    (* Qed. *)
+    Admitted.
+
+    Lemma sound_exec_block_addr {instrs ainstr apc} Φ (h : SCHeap) :
+      cexec_block_addr instrs ainstr apc Φ h ->
+      interpret_scheap h ∗ lptsreg pc apc ∗ (∃ v, lptsreg nextpc v) ∗ ptsto_instrs ainstr instrs ⊢
+      (∀ an, lptsreg pc an ∗ (∃ v, lptsreg nextpc v) ∗ ptsto_instrs ainstr instrs ∗
+             (∃ h', interpret_scheap h' ∧ ⌜Φ an h'⌝) -∗ WP_loop) -∗ WP_loop.
+    Proof.
+      revert ainstr apc Φ h.
+      induction instrs as [|instr instrs]; cbn; intros ainstr apc Φ h;
+        cbv [bind assert_formula lift_purespec CPureSpec.assert_formula
+               CPureSpec.assert_pathcondition pure CPureSpec.pure].
+      - intros HΦ. iIntros "(Hpre & Hpc & Hnpc & _) Hk".
+        iApply "Hk"; iFrame; auto.
+      - intros [-> Hverif%sound_exec_instruction].
+        unfold semTripleOneInstrStep, semTTriple in Hverif.
+        iIntros "(Hh & Hpc & Hnpc & Hinstr & Hinstrs) Hk".
+        iApply semWP_seq.
+        iApply semWP_call_inline.
+        iApply (semWP_mono with "[-Hinstrs Hk] [Hinstrs Hk]").
+        iApply semTWP_semWP. iApply Hverif. iFrame. clear Hverif.
+        cbn.
+        iIntros ([v|m] _); last (iIntros "_"; now rewrite semWP_fail);
+          iIntros "([%an (Hnpc & Hpc & Hk2)] & Hinstr)".
+        iDestruct "Hk2" as "(%h' & Hh' & %Hexec)".
+        specialize (IHinstrs _ _ _ _ Hexec). clear Hexec.
+        iApply (semWP_call_inline loop).
+        iApply (IHinstrs with "[$Hh' $Hpc Hnpc $Hinstrs]").
+        { now iExists an. }
+        iIntros (an2) "(Hpc & Hnpc & Hinstrs & HPOST)".
+        iApply ("Hk" with "[$]").
+    Qed.
+
+    Lemma sound_cexec_triple_addr {Γ : LCtx} {pre post instrs} {ι : Valuation Γ} :
+      cexec_triple_addr pre instrs post (fun _ _ => True) []%list ->
+      ⊢ semTripleBlock (λ a : Val ty_word, asn.interpret pre (ι.[("a"::ty_xlenbits) ↦ a])) instrs
+          (λ a na : Val ty_word, asn.interpret post (ι.[("a"::ty_xlenbits) ↦ a].[("an"::ty_xlenbits) ↦ na])).
+    Proof.
+      cbv [cexec_triple_addr bind demonic_ctx demonic CPureSpec.demonic lift_purespec].
+      iIntros (Htrip a) "(Hpre & Hpc & Hnpc & Hinstrs) Hk".
+      rewrite CPureSpec.wp_demonic_ctx in Htrip.
+      specialize (Htrip ι a). apply produce_sound in Htrip.
+      iPoseProof (Htrip with "[$] Hpre") as "(%h2 & [Hh2 %Hexec])". clear Htrip.
+      apply sound_exec_block_addr in Hexec.
+      iApply (Hexec with "[$]"). clear Hexec.
+      iIntros (an2) "(Hpc & Hnpc & Hinstrs & (%h3 & [Hh3 %Hconsume]))".
+      apply consume_sound in Hconsume.
+      iPoseProof (Hconsume with "Hh3") as "[HPOST Hheap]".
+      iApply ("Hk" with "[$]").
+    Qed.
+
+    Lemma sound_cblock_verification_condition {Γ pre post instrs} :
+      cblock_verification_condition pre instrs post ->
+      forall ι : Valuation Γ,
+      ⊢ semTripleBlock (fun a => asn.interpret pre (ι.[("a"::ty_xlenbits) ↦ a]))
+          instrs
+          (fun a na => asn.interpret post (ι.[("a"::ty_xlenbits) ↦ a].[("an"::ty_xlenbits) ↦ na])).
+    Proof.
+      intros Hverif ι.
+      now apply sound_cexec_triple_addr.
+    Qed.
+
+    Lemma sound_sblock_verification_condition {Γ pre post instrs} :
+      safeE (postprocess (sblock_verification_condition pre instrs post wnil)) ->
+      forall ι : Valuation Γ,
+      ⊢ semTripleBlock (fun a => asn.interpret pre (ι.[("a"::ty_xlenbits) ↦ a]))
+          instrs
+          (fun a na => asn.interpret post (ι.[("a"::ty_xlenbits) ↦ a].[("an"::ty_xlenbits) ↦ na])).
+    Proof.
+      intros Hverif ι.
+      apply sound_cexec_triple_addr.
+      apply (safeE_safe env.nil), postprocess_sound in Hverif.
+      apply LogicalSoundness.psafe_safe in Hverif; [|done].
+      revert Hverif.
+      apply rexec_triple_addr.
+      - easy.
+      - easy.
+      - easy.
+      - constructor.
+    Qed.
+
+  End Soundness.
+
+End BlockVerificationDerived.
+
+Section AnnotatedBlockVerification.
+
+  Inductive AnnotInstr :=
+  | AnnotAST  (i : AST)
+  | AnnotDebugBreak
+  | AnnotLemmaInvocation {Δ} (l : 𝑳 Δ) (es : NamedEnv (Exp [ctx]) Δ)
+  .
+
+  Section Debug.
+
+    Import option.notations.
+
+    Record DebugBlockver (Σ : LCtx) : Type :=
+      MkDebugBlockver
+        { debug_blockver_pathcondition          : PathCondition Σ;
+          debug_blockver_heap                   : SHeap Σ;
+        }.
+    #[export] Instance SubstDebugBlockver : Subst DebugBlockver :=
+      fun Σ0 d Σ1 ζ01 =>
+        match d with
+        | MkDebugBlockver pc1 h => MkDebugBlockver (subst pc1 ζ01) (subst h ζ01)
+        end.
+
+    #[export] Instance SubstLawsDebugBlockver : SubstLaws DebugBlockver.
+    Proof.
+      constructor.
+      - intros ? []; cbn; now rewrite ?subst_sub_id.
+      - intros ? ? ? ? ? []; cbn; now rewrite ?subst_sub_comp.
+    Qed.
+
+    #[export] Instance OccursCheckDebugBlockver : OccursCheck DebugBlockver :=
+      fun Σ x xIn d =>
+        match d with
+        | MkDebugBlockver pc1 h =>
+            pc' <- occurs_check xIn pc1 ;;
+            h'  <- occurs_check xIn h ;;
+            Some (MkDebugBlockver pc' h')
+        end.
+
+  End Debug.
+
+  Import RiscvPmpBlockVerifSpec.
+
+  Section Symbolic.
+
+    Import ModalNotations.
+    Import SHeapSpec.
+    Import SHeapSpec.notations.
+
+    Fixpoint sexec_annotated_block_addr (b : list AnnotInstr) :
+      ⊢ STerm ty_xlenbits -> STerm ty_xlenbits -> SHeapSpec (STerm ty_xlenbits) :=
+      fun w0 ainstr apc =>
+        match b with
+        | nil       => pure apc
+        | cons instr b' =>
+            match instr with
+            | AnnotAST i =>
+                ⟨ θ1 ⟩ _    <- assert_formula
+                                 (fun _ => amsg.empty)
+                                 (formula_relop bop.eq ainstr apc) ;;
+                ⟨ θ2 ⟩ apc' <- sexec_instruction i (persist__term apc θ1) ;;
+                sexec_annotated_block_addr b'
+                  (term_binop bop.bvadd
+                     (persist__term ainstr (θ1 ∘ θ2))
+                     (term_val ty_word bv_instrsize))
+                  apc'
+            | AnnotDebugBreak =>
+                debug
+                  (fun (h0 : SHeap w0) =>
+                     amsg.mk
+                       {| debug_blockver_pathcondition := wco w0;
+                          debug_blockver_heap := h0
+                       |})
+                  (pure apc)
+            | AnnotLemmaInvocation l es =>
+                let args := seval_exps [env] es in
+                ⟨ θ1 ⟩ _ <- call_lemma (LEnv l) args ;;
+                sexec_annotated_block_addr b'
+                  (persist__term ainstr θ1)
+                  (persist__term apc θ1)
+            end
+        end.
+
+    Definition sexec_annotated_block_triple_addr {Σ : LCtx}
+      (req : Assertion (Σ ▻ ("a"::ty_xlenbits))) (b : list AnnotInstr)
+      (ens : Assertion (Σ ▻ ("a"::ty_xlenbits) ▻ ("an"::ty_xlenbits))) :
+      ⊢ SHeapSpec Unit :=
+      fun _ =>
+        ⟨ θ1 ⟩ lenv1 <- demonic_ctx id Σ ;;
+        ⟨ θ2 ⟩ a2 <- demonic (Some "a") _ ;;
+        let lenv2 := env.snoc (persist (A := Sub Σ) lenv1 θ2) _ a2 in
+        ⟨ θ3 ⟩ _ <- produce req lenv2 ;;
+        let a3 := persist__term a2 θ3 in
+        ⟨ θ4 ⟩ na <- sexec_annotated_block_addr b a3 a3 ;;
+        let lenv4 := persist lenv2 (θ3 ∘ θ4) in
+        consume ens lenv4.["an"∷ty_xlenbits ↦ na].
+
+    (* This is a VC for triples, for doubles we probably need to talk
+     about the continuation of a block. *)
+    Definition sannotated_block_verification_condition {Σ : LCtx}
+      (req : Assertion (Σ ▻ "a"∷ty_xlenbits)) (b : list AnnotInstr)
+      (ens : Assertion (Σ ▻ "a"∷ty_xlenbits ▻ "an"∷ty_xlenbits)) : ⊢ 𝕊 :=
+      (* SHeapSpec does not perform a leakcheck. We could include one here. *)
+      fun w => SHeapSpec.run (sexec_annotated_block_triple_addr req b ens (w := w)).
+
+  End Symbolic.
+
+  Section Shallow.
+
+    Import CHeapSpec CHeapSpec.notations.
+
+    Fixpoint cexec_annotated_block_addr (b : list AnnotInstr) :
+      Val ty_xlenbits -> Val ty_xlenbits -> CHeapSpec (Val ty_xlenbits) :=
+      fun ainstr apc =>
+        match b with
+        | nil       => pure apc
+        | cons instr b' =>
+            match instr with
+            | AnnotAST i =>
+                _ <- assert_formula (ainstr = apc) ;;
+                apc' <- cexec_instruction i apc ;;
+                cexec_annotated_block_addr b' (bv.add ainstr bv_instrsize) apc'
+            | AnnotDebugBreak => debug (pure apc)
+            | AnnotLemmaInvocation l es =>
+                let args := evals es [env] in
+                _ <- call_lemma (LEnv l) args ;;
+                cexec_annotated_block_addr b' ainstr apc
+            end
+        end.
+
+    Definition cexec_annotated_block_triple_addr {Σ}
+      (req : Assertion (Σ ▻ "a"∷ty_xlenbits)) (b : list AnnotInstr)
+      (ens : Assertion (Σ ▻ "a"∷ty_xlenbits ▻ "an"∷ty_xlenbits)) :
+      CHeapSpec unit :=
+      lenv <- demonic_ctx Σ ;;
+      a  <- demonic _ ;;
+      _  <- produce req lenv.["a"∷ty_xlenbits ↦ a]  ;;
+      na <- cexec_annotated_block_addr b a a ;;
+      consume ens lenv.["a"∷ty_xlenbits ↦ a].["an"∷ty_xlenbits ↦ na].
+
+    Definition cannotated_block_verification_condition {Σ : LCtx}
+      (req : Assertion (Σ ▻ "a"∷ty_xlenbits)) (b : list AnnotInstr)
+      (ens : Assertion (Σ ▻ "a"∷ty_xlenbits ▻ "an"∷ty_xlenbits)) : Prop :=
+      (* SHeapSpec does not perform a leakcheck. We could include one here. *)
+      CHeapSpec.run (cexec_annotated_block_triple_addr req b ens).
+
+    #[export] Instance mono_cexec_annotated_block_addr {instrs ainstr apc} :
+      Monotonic (MHeapSpec eq) (cexec_annotated_block_addr instrs ainstr apc).
+    Proof.
+      revert ainstr apc.
+      induction instrs; cbn; try typeclasses eauto.
+      destruct a; typeclasses eauto.
+    Qed.
+
+  End Shallow.
+
+  Section Relational.
+
+    Import RiscvPmpIrisInstanceWithContracts.
+    Import RiscvPmpIrisInstanceWithContracts.StoreSpec.
+    Import logicalrelation logicalrelation.notations.
+    Import proofmode.
+    Import iris.proofmode.tactics.
+    Import RiscvPmpSignature.HeapSpec.
+    Import RSolve.
+
+    Lemma rexec_annotated_block_addr (b : list AnnotInstr) {w} :
+      ⊢ ℛ⟦RVal ty_xlenbits -> RVal ty_xlenbits -> RHeapSpec (RVal ty_xlenbits)⟧
+          (cexec_annotated_block_addr b)
+          (sexec_annotated_block_addr b (w := w)).
+    Proof.
+      iAssert (ℛ⟦□ᵣ (RVal ty_xlenbits -> RVal ty_xlenbits -> RHeapSpec (RVal ty_xlenbits))⟧
+                 (cexec_annotated_block_addr b)
+                 (fun w' θ => sexec_annotated_block_addr b (w := w'))) as "H".
+      { iInduction b as [|instr b] "IHb"; rsolve.
+        destruct instr; cbn; rsolve.
+        - iApply "IHb"; rsolve.
+        - iApply "IHb"; rsolve.
+      }
+      now iApply (unconditionally_T with "H").
+    Qed.
+
+    Lemma rexec_annotated_block_triple_addr {Σ}
+      (req : Assertion (Σ ▻ "a"∷ty_xlenbits)) (b : list AnnotInstr)
+      (ens : Assertion (Σ ▻ "a"∷ty_xlenbits ▻ "an"∷ty_xlenbits)) {w} :
+      ⊢ ℛ⟦RHeapSpec RUnit⟧
+          (cexec_annotated_block_triple_addr req b ens)
+          (sexec_annotated_block_triple_addr req b ens (w := w)).
+    Proof.
+      unfold cexec_annotated_block_triple_addr, sexec_annotated_block_triple_addr.
+      rsolve.
+      iApply rexec_annotated_block_addr; rsolve.
+      rewrite !forgetting_trans.
+      iModIntro.
+      iModIntro.
+      rsolve.
+    Qed.
+
+    Lemma rannotated_block_verification_condition {Σ}
+      (req : Assertion (Σ ▻ "a"∷ty_xlenbits)) (b : list AnnotInstr)
+      (ens : Assertion (Σ ▻ "a"∷ty_xlenbits ▻ "an"∷ty_xlenbits)) {w} :
+      ⊢ ℛ⟦LogicalSoundness.RProp⟧
+          (cannotated_block_verification_condition req b ens)
+          (sannotated_block_verification_condition req b ens w).
+    Proof.
+      iApply HeapSpec.refine_run.
+      iApply rexec_annotated_block_triple_addr.
+    Qed.
+
+  End Relational.
+
+  Section Soundness.
+
+    Import iris.base_logic.lib.iprop iris.proofmode.tactics.
+    Import RiscvPmpIrisInstanceWithContracts.
+    Import ProgramLogic.
+    Import CHeapSpec.
+
+    Context {Σ} {GS : sailGS Σ}.
+
+    Definition extract_AST (i : AnnotInstr) : option AST :=
+      match i with
+      | AnnotAST a => Some a
+      | _ => None
+      end.
+
+    Lemma sound_exec_annotated_block_addr {instrs ainstr apc} (h : SCHeap) (POST : Val ty_xlenbits -> iProp Σ) :
+      LemmaSem ->
+      cexec_annotated_block_addr instrs ainstr apc (fun res h' => interpret_scheap h' ⊢ POST res) h ->
+      ⊢ ((interpret_scheap h ∗ lptsreg pc apc ∗ (∃ v, lptsreg nextpc v) ∗ ptsto_instrs ainstr (omap extract_AST instrs)) -∗
+         (∀ an, lptsreg pc an ∗ (∃ v, lptsreg nextpc v) ∗ ptsto_instrs ainstr (omap extract_AST instrs) ∗ POST an -∗ WP_loop) -∗
+         WP_loop)%I.
+    Proof.
+      intros lemSem.
+      revert ainstr apc h POST.
+      induction instrs as [|instr instrs]; cbn; intros ainstr apc h POST.
+      - iIntros (->) "(Hpre & Hpc & Hnpc & _) Hk".
+        iApply "Hk"; iFrame.
+      - cbv [bind assert_formula lift_purespec CPureSpec.assert_formula
+               CPureSpec.assert_pathcondition].
+        destruct instr as [instr| |Δ lem es].
+        + intros [-> Hverif]. cbn [extract_AST ptsto_instrs].
+          iIntros "(Hh & Hpc & Hnpc & Hinstr & Hinstrs) Hk".
+          iApply semWP_seq.
+          iApply semWP_call_inline.
+          iApply (semWP_mono with "[Hh Hnpc Hpc Hinstr]").
+          { iApply semTWP_semWP. iApply (sound_exec_instruction Hverif). iFrame. }
+          clear Hverif.
+          iIntros ([v|m] _); last (iIntros "_"; now rewrite semWP_fail);
+            iIntros "([%an (Hnpc & Hpc & (%h2 & Hh2 & %Hverif))] & Hinstr)".
+          iApply (semWP_call_inline loop).
+          specialize (IHinstrs _ _ _ _ Hverif).
+          iApply (IHinstrs with "[$Hh2 $Hpc Hnpc $Hinstrs]").
+          by iExists _.
+          iIntros (an2) "(Hpc & Hnpc & Hinstrs & HPOST)".
+          iApply ("Hk" with "[$]").
+        + cbv [debug pure lift_purespec CPureSpec.pure].
+          iIntros (->) "(Hh & Hpc & Hnpc & Hinstrs) Hk".
+          now iApply ("Hk" with "[$Hpc $Hnpc $Hinstrs Hh]").
+        + iIntros (Hlemcall) "(Hh & Hpc & Hnpc & Hinstrs) Hk".
+          pose proof (Hlem := lemSem _ lem).
+          apply call_lemma_sound in Hlemcall. destruct Hlemcall. cbn in *.
+          iPoseProof (H with "Hh") as "(%ι & %Heq & Hreq & Hk2)". clear H.
+          iPoseProof (Hlem with "Hreq") as "Hens".
+          iPoseProof ("Hk2" with "Hens") as "(%h' & Hh' & %Hk2)".
+          apply IHinstrs in Hk2.
+          iApply (Hk2 with "[$Hh' $Hpc $Hnpc $Hinstrs] Hk").
+    Qed.
+
+    Definition semTripleAnnotatedBlock (PRE : Val ty_word -> iProp Σ)
+      (instrs : list AnnotInstr) (POST : Val ty_word -> Val ty_word -> iProp Σ) : iProp Σ :=
+      (∀ a,
+         (PRE a ∗ pc ↦ a ∗ (∃ v, nextpc ↦ v) ∗ ptsto_instrs a (omap extract_AST instrs)) -∗
+         (∀ an, pc ↦ an ∗ (∃ v, nextpc ↦ v) ∗ ptsto_instrs a (omap extract_AST instrs) ∗ POST a an -∗ WP_loop) -∗
+         WP_loop)%I.
+    Global Arguments semTripleAnnotatedBlock PRE%_I instrs POST%_I.
+
+    Lemma sound_cexec_annotated_block_triple_addr {Γ pre post instrs} :
+      LemmaSem ->
+      (cexec_annotated_block_triple_addr (Σ := Γ) pre instrs post (λ _ _ , True) []%list) ->
+      forall ι : Valuation Γ,
+      ⊢ semTripleAnnotatedBlock (λ a : Val ty_word, asn.interpret pre (ι.[("a"::ty_xlenbits) ↦ a])) instrs
+          (λ a na : Val ty_word, asn.interpret post (ι.[("a"::ty_xlenbits) ↦ a].[("an"::ty_xlenbits) ↦ na])).
+    Proof.
+      intros lemSem Hexec ι.
+      iIntros (a) "(Hpre & Hpc & Hnpc & Hinstrs) Hk".
+      hnf in Hexec.
+      rewrite CPureSpec.wp_demonic_ctx in Hexec.
+      specialize (Hexec ι a).
+      unfold bind in Hexec.
+      iPoseProof (produce_sound _ _ Hexec with "[//] [$Hpre]") as "(%h2 & Hh2 & %Hexec')".
+      clear Hexec.
+      iApply (sound_exec_annotated_block_addr (apc := a) h2 with "[$Hh2 $Hpc $Hnpc $Hinstrs]"); auto.
+      revert Hexec'.
+      apply mono_cexec_annotated_block_addr.
+      intros ? ? <- h3 Hcons.
+      iIntros "Hh3".
+      iPoseProof (consume_sound _ _ Hcons with "Hh3") as "[Hcons _]".
+      iFrame.
+    Qed.
+
+    Lemma sound_sannotated_block_verification_condition {Γ pre post instrs} :
+      LemmaSem ->
+      safeE (postprocess (sannotated_block_verification_condition (Σ := Γ)
+                            pre instrs post wnil)) ->
+      forall ι : Valuation Γ,
+      ⊢ semTripleAnnotatedBlock (fun a => asn.interpret pre (ι.[("a"::ty_xlenbits) ↦ a]))
+          instrs (fun a na => asn.interpret post (ι.[("a"::ty_xlenbits) ↦ a].[("an"::ty_xlenbits) ↦ na])).
+    Proof.
+      unfold sannotated_block_verification_condition, SHeapSpec.run.
+      intros lemSem Hverif ι.
+      apply sound_cexec_annotated_block_triple_addr; auto.
+      apply (safeE_safe env.nil), postprocess_sound in Hverif.
+      apply LogicalSoundness.psafe_safe in Hverif; [|done].
+      revert Hverif.
+      apply rexec_annotated_block_triple_addr.
+      - easy.
+      - easy.
+      - easy.
+      - constructor.
+    Qed.
+
+  End Soundness.
+
+End AnnotatedBlockVerification.
