theories/Program.v
@@ -556,7 +556,7 @@ End ProgramMixin.
 Module Type WellFoundedKit (B : Base) (FDecl : FunDecl B) (FDK : FunDefKit B FDecl)
   (Import PM : ProgramMixin B FDecl FDK).
 
-  Parameter Inline 𝑭_well_founded : exists (fuel : nat), well_founded (InvokedByFunPackage fuel).
+  Parameter Inline 𝑭_well_founded : well_founded (InvokedByFunPackage FDecl.inline_fuel).
 End WellFoundedKit.
 
 Module Type Program (B : Base) :=
